PropositionalLogic/KripkeSemantics.v
@@ -1,8 +1,8 @@
 Require Import Coq.Logic.Classical_Prop.
 Require Import Coq.Classes.RelationClasses.
+Require Import Coq.Relations.Relation_Definitions.
 Require Import Logic.LogicBase.
 Require Import Logic.MinimunLogic.MinimunLogic.
-Require Import Logic.MinimunLogic.SyntacticReduction.
 Require Import Logic.PropositionalLogic.Syntax.
 
 Local Open Scope logic_base.
@@ -16,7 +16,7 @@ Class PreKripkeSemantics (L: Language) (SM: Semantics L): Type := {
 
 Notation "'KRIPKE:'  M , m" := (build_model M m) (at level 59, no associativity) : logic_base.
 
-Class KripkeIntuitionisticSemantics (L: Language) {nL: NormalLanguage L} {pL: PropositionalLanguage L} (SM: Semantics L) {icSM: ReductionConsistentSemantics IntuitionisticReduction SM} {pkSM: PreKripkeSemantics L SM}: Type := {
+Class KripkeIntuitionisticSemantics (L: Language) {nL: NormalLanguage L} {pL: PropositionalLanguage L} (SM: Semantics L) {pkSM: PreKripkeSemantics L SM}: Type := {
   Korder: forall {M: Kmodel}, Kworlds M -> Kworlds M -> Prop; (* <= *)
   sat_mono: forall M m n x, Korder m n -> KRIPKE: M , n |= x -> KRIPKE: M , m |= x;
   sat_impp: forall M m x y, KRIPKE: M , m |= x --> y <-> (forall n, Korder n m -> KRIPKE: M , n |= x -> KRIPKE: M , n |= y);
@@ -84,77 +84,9 @@ Definition denotation {Var: Type} (F: frame) (eval: Var -> sem F): expr Var -> s
   | andp y z => sem_and (denotation y) (denotation z)
   | orp y z => sem_or (denotation y) (denotation z)
   | impp y z => sem_imp (denotation y) (denotation z)
-  | iffp y z => sem_iff (denotation y) (denotation z)
-  | negp y => sem_neg (denotation y)
-  | truep => sem_true
   | falsep => sem_false
   | varp p => eval p
   end.
-
-Lemma ImpAndOrAsPrime_consistent {Var: Type}:
-  forall x y: expr Var,
-    @ImpAndOrAsPrime.atomic_reduce (L Var) (nL Var) (pL Var) x y ->
-    forall f eval v, proj1_sig (denotation f eval x) v <-> proj1_sig (denotation f eval y) v.
-Proof.
-  intros; split; intros; destruct H; auto.
-Qed.
-
-Lemma ReduceIff_consistent {Var: Type}:
-  forall x y: expr Var,
-    @ReduceIff.atomic_reduce (L Var) (nL Var) (pL Var) x y ->
-    forall f eval v, proj1_sig (denotation f eval x) v <-> proj1_sig (denotation f eval y) v.
-Proof.
-  intros; split; intros; destruct H; auto.
-Qed.
-
-Lemma ReduceTrue_consistent {Var: Type}:
-  forall x y: expr Var,
-    @ReduceTrue.atomic_reduce (L Var) (nL Var) (pL Var) x y ->
-    forall f eval v, proj1_sig (denotation f eval x) v <-> proj1_sig (denotation f eval y) v.
-Proof.
-  intros; split; intros; destruct H.
-  + hnf; intros; auto.
-  + hnf; auto.
-Qed.
-
-Lemma RPC_aux {Var: Type}: forall  F eval (x y: expr Var) sp,
-  (forall v, proj1_sig (denotation F eval x) v <-> proj1_sig (denotation F eval y) v) ->
-  (forall v, proj1_sig (denotation F eval (single_propagation_denote sp x)) v <->
-             proj1_sig (denotation F eval (single_propagation_denote sp y)) v).
-Proof.
-  intros.
-  destruct sp; intros.
-  + specialize (H v).
-    simpl in *.
-    tauto.
-  + specialize (H v).
-    simpl in *.
-    tauto.
-  + specialize (H v).
-    simpl in *.
-    tauto.
-  + specialize (H v).
-    simpl in *.
-    tauto.
-  + simpl in *.
-    split; intros HH u Hu; specialize (HH u Hu); specialize (H u); tauto.
-  + simpl in *.
-    split; intros HH u Hu; specialize (HH u Hu); specialize (H u); tauto.
-  + simpl in *.
-    apply Morphisms_Prop.and_iff_morphism.
-    - simpl in *.
-      split; intros HH u Hu; specialize (HH u Hu); specialize (H u); tauto.
-    - simpl in *.
-      split; intros HH u Hu; specialize (HH u Hu); specialize (H u); tauto.
-  + simpl in *.
-    apply Morphisms_Prop.and_iff_morphism.
-    - simpl in *.
-      split; intros HH u Hu; specialize (HH u Hu); specialize (H u); tauto.
-    - simpl in *.
-      split; intros HH u Hu; specialize (HH u Hu); specialize (H u); tauto.
-  + simpl in *.
-    split; intros HH u Hu; specialize (HH u Hu); specialize (H u); tauto.
-Qed.
 
 End KripkeSemantics.
 
@@ -182,27 +114,6 @@ Instance SM (Var: Type): Semantics (PropositionalLanguage.L Var) :=
 Local Open Scope logic_base.
 Local Open Scope PropositionalLogic.
 
-Lemma RPC {Var: Type}: ReductionPropagationConsistentSemantics (SM Var).
-Proof.
-  hnf; intros; simpl in *.
-  destruct m as [M v].
-  pose proof (fun v => H (Build_model _ M v)).
-  revert v; simpl in H0; clear H. simpl.
-  apply RPC_aux; auto.
-Qed.
-
-Instance icSM (Var: Type): ReductionConsistentSemantics IntuitionisticReduction (SM Var).
-Proof.
-  apply Build_ReductionConsistentSemantics.
-  + hnf; intros.
-    revert x y H m.
-    repeat apply disjunction_reduce_consistent_semantics; intros.
-    - apply ImpAndOrAsPrime_consistent; auto.
-    - apply ReduceIff_consistent; auto.
-    - apply ReduceTrue_consistent; auto.
-  + apply RPC.
-Qed.
-
 Instance pkSM (Var: Type): PreKripkeSemantics (PropositionalLanguage.L Var) (SM Var) :=
   Build_PreKripkeSemantics _ (SM Var)
    Kmodel
@@ -211,7 +122,7 @@ Instance pkSM (Var: Type): PreKripkeSemantics (PropositionalLanguage.L Var) (SM 
 
 Instance kiSM (Var: Type): KripkeIntuitionisticSemantics (PropositionalLanguage.L Var) (SM Var).
 Proof.
-  apply (Build_KripkeIntuitionisticSemantics _ _ _ _ _ (pkSM Var) (fun M => Korder M)).
+  apply (Build_KripkeIntuitionisticSemantics _ _ _ _ (pkSM Var) (fun M => Korder M)).
   + hnf; simpl; intros.
     eapply (proj2_sig (denotation M (Kvar M) x)); eauto.
   + split; auto.
@@ -249,27 +160,6 @@ Instance SM (Var: Type): Semantics (PropositionalLanguage.L Var) :=
 Local Open Scope logic_base.
 Local Open Scope PropositionalLogic.
 
-Lemma RPC {Var: Type}: ReductionPropagationConsistentSemantics (SM Var).
-Proof.
-  hnf; intros; simpl in *.
-  destruct m as [M v].
-  pose proof (fun v => H (Build_model _ M v)).
-  revert v; simpl in H0; clear H. simpl.
-  apply RPC_aux; auto.
-Qed.
-
-Instance icSM (Var: Type): ReductionConsistentSemantics IntuitionisticReduction (SM Var).
-Proof.
-  apply Build_ReductionConsistentSemantics.
-  + hnf; intros.
-    revert x y H m.
-    repeat apply disjunction_reduce_consistent_semantics; intros.
-    - apply ImpAndOrAsPrime_consistent; auto.
-    - apply ReduceIff_consistent; auto.
-    - apply ReduceTrue_consistent; auto.
-  + apply RPC.
-Qed.
-
 Instance pkSM (Var: Type): PreKripkeSemantics (PropositionalLanguage.L Var) (SM Var) :=
   Build_PreKripkeSemantics _ (SM Var)
    Kmodel
@@ -278,7 +168,7 @@ Instance pkSM (Var: Type): PreKripkeSemantics (PropositionalLanguage.L Var) (SM 
 
 Instance kiSM (Var: Type): KripkeIntuitionisticSemantics (PropositionalLanguage.L Var) (SM Var).
 Proof.
-  apply (Build_KripkeIntuitionisticSemantics _ _ _ _ _ (pkSM Var) (fun M => Korder M)).
+  apply (Build_KripkeIntuitionisticSemantics _ _ _ _ (pkSM Var) (fun M => Korder M)).
   + hnf; simpl; intros.
     eapply (proj2_sig (denotation M (Kvar M) x)); eauto.
   + split; auto.
