PropositionalLogic/Syntax.v
@@ -3,40 +3,15 @@ Require Import Logic.lib.Bijection.
 Require Import Logic.lib.Countable.
 Require Import Logic.LogicBase.
 Require Import Logic.MinimunLogic.MinimunLogic.
-Require Import Logic.MinimunLogic.SyntacticReduction.
 
 Class PropositionalLanguage (L: Language) {nL: NormalLanguage L}: Type := {
   andp : expr -> expr -> expr;
-  orp : expr -> expr -> expr;
-  iffp : expr -> expr -> expr;
-  negp : expr -> expr;
-  truep : expr;
-  and1_propag: expr -> single_propagation;
-  and2_propag: expr -> single_propagation;
-  or1_propag: expr -> single_propagation;
-  or2_propag: expr -> single_propagation;
-  iff1_propag: expr -> single_propagation;
-  iff2_propag: expr -> single_propagation;
-  neg_propag: single_propagation;
-  and1_propag_denote: forall x y, single_propagation_denote (and1_propag x) y = andp y x;
-  and2_propag_denote: forall x y, single_propagation_denote (and2_propag x) y = andp x y;
-  or1_propag_denote: forall x y, single_propagation_denote (or1_propag x) y = orp y x;
-  or2_propag_denote: forall x y, single_propagation_denote (or2_propag x) y = orp x y;
-  iff1_propag_denote: forall x y, single_propagation_denote (iff1_propag x) y = iffp y x;
-  iff2_propag_denote: forall x y, single_propagation_denote (iff2_propag x) y = iffp x y;
-  neg_propag_denote: forall x, single_propagation_denote neg_propag x = negp x
+  orp : expr -> expr -> expr
 }.
 
-Inductive PropositionalPropag {L: Language} {nL: NormalLanguage L} {pL: PropositionalLanguage L}: single_propagation -> Prop :=
-  | imp1_prop_propag: forall x: expr, PropositionalPropag (imp1_propag x)
-  | imp2_prop_propag: forall x: expr, PropositionalPropag (imp2_propag x)
-  | and1_prop_propag: forall x: expr, PropositionalPropag (and1_propag x)
-  | and2_prop_propag: forall x: expr, PropositionalPropag (and2_propag x)
-  | or1_prop_propag: forall x: expr, PropositionalPropag (or1_propag x)
-  | or2_prop_propag: forall x: expr, PropositionalPropag (or2_propag x)
-  | iff1_prop_propag: forall x: expr, PropositionalPropag (iff1_propag x)
-  | iff2_prop_propag: forall x: expr, PropositionalPropag (iff2_propag x)
-  | neg_prop_propag: PropositionalPropag neg_propag.
+Definition negp {L: Language} {nL: NormalLanguage L} (x: expr): expr := impp x falsep.
+Definition iffp {L: Language} {nL: NormalLanguage L} {pL: PropositionalLanguage L} (x y: expr): expr := andp (impp x y) (impp y x).
+Definition truep {L: Language} {nL: NormalLanguage L}: expr := impp falsep falsep.
 
 Notation "x && y" := (andp x y) (at level 40, left associativity) : PropositionalLogic.
 Notation "x || y" := (orp x y) (at level 50, left associativity) : PropositionalLogic.
@@ -47,127 +22,6 @@ Notation "'TT'" := truep : PropositionalLogic.
 Local Open Scope logic_base.
 Local Open Scope PropositionalLogic.
 
-Definition PropositonalPropagationConsistentProvable {L: Language} {nL: NormalLanguage L} {pL: PropositionalLanguage L} (Gamma: ProofTheory L): Prop :=
-  forall x y sp,
-    PropositionalPropag sp ->
-    (|-- x --> y /\ |-- y --> x) ->
-    (|-- single_propagation_denote sp x --> single_propagation_denote sp y /\
-     |-- single_propagation_denote sp y --> single_propagation_denote sp x).
-
-Lemma and_reduce {L: Language} {nL: NormalLanguage L} {pL: PropositionalLanguage L} {R: SyntacticReduction L}:
-  forall x1 x2 y1 y2,
-    reduce x1 x2 ->
-    reduce y1 y2 ->
-    reduce (x1 && y1) (x2 && y2).
-Proof.
-  intros.
-  eapply reduce_trans.
-  + apply propag_reduce_reduce.
-    rewrite <- and1_propag_denote.
-    apply (propag_reduce_spec _ _ _ (and1_propag y1 :: nil) H).
-  + simpl; rewrite and1_propag_denote.
-    apply propag_reduce_reduce.
-    rewrite <- !and2_propag_denote.
-    apply (propag_reduce_spec _ _ _ (and2_propag x2 :: nil) H0).
-Qed.
-
-Lemma or_reduce {L: Language} {nL: NormalLanguage L} {pL: PropositionalLanguage L} {R: SyntacticReduction L}:
-  forall x1 x2 y1 y2,
-    reduce x1 x2 ->
-    reduce y1 y2 ->
-    reduce (x1 || y1) (x2 || y2).
-Proof.
-  intros.
-  eapply reduce_trans.
-  + apply propag_reduce_reduce.
-    rewrite <- or1_propag_denote.
-    apply (propag_reduce_spec _ _ _ (or1_propag y1 :: nil) H).
-  + simpl; rewrite or1_propag_denote.
-    apply propag_reduce_reduce.
-    rewrite <- !or2_propag_denote.
-    apply (propag_reduce_spec _ _ _ (or2_propag x2 :: nil) H0).
-Qed.
-
-Lemma iff_reduce {L: Language} {nL: NormalLanguage L} {pL: PropositionalLanguage L} {R: SyntacticReduction L}:
-  forall x1 x2 y1 y2,
-    reduce x1 x2 ->
-    reduce y1 y2 ->
-    reduce (x1 <--> y1) (x2 <--> y2).
-Proof.
-  intros.
-  eapply reduce_trans.
-  + apply propag_reduce_reduce.
-    rewrite <- iff1_propag_denote.
-    apply (propag_reduce_spec _ _ _ (iff1_propag y1 :: nil) H).
-  + simpl; rewrite iff1_propag_denote.
-    apply propag_reduce_reduce.
-    rewrite <- !iff2_propag_denote.
-    apply (propag_reduce_spec _ _ _ (iff2_propag x2 :: nil) H0).
-Qed.
-
-Lemma neg_reduce {L: Language} {nL: NormalLanguage L} {pL: PropositionalLanguage L} {R: SyntacticReduction L}:
-  forall x1 x2, reduce x1 x2 -> reduce (~~ x1) (~~ x2).
-Proof.
-  intros.
-  apply propag_reduce_reduce.
-  rewrite <- !neg_propag_denote.
-  apply (propag_reduce_spec _ _ _ (neg_propag :: nil) H).
-Qed.
-
-Module ImpNegAsPrime.
-
-Inductive atomic_reduce {L: Language} {nL: NormalLanguage L} {pL: PropositionalLanguage L}: expr -> expr -> Prop :=
-| andp_reduce: forall x y, atomic_reduce (x && y) (~~ (x --> ~~ y))
-| orp_reduce: forall x y, atomic_reduce (x || y) (~~ x --> y)
-.
-
-End ImpNegAsPrime.
-
-Module ImpAndOrAsPrime.
-
-Inductive atomic_reduce {L: Language} {nL: NormalLanguage L} {pL: PropositionalLanguage L}: expr -> expr -> Prop :=
-| negp_reduce: forall x, atomic_reduce (~~ x) (x --> FF)
-.
-
-End ImpAndOrAsPrime.
-
-Module ReduceIff.
-
-Inductive atomic_reduce {L: Language} {nL: NormalLanguage L} {pL: PropositionalLanguage L}: expr -> expr -> Prop :=
-| iff_reduce: forall x y, atomic_reduce (x <--> y) ((x --> y) && (y --> x)).
-
-End ReduceIff.
-
-Module ReduceFalse.
-
-Inductive atomic_reduce {L: Language} {nL: NormalLanguage L} {pL: PropositionalLanguage L}: expr -> expr -> Prop :=
-| falsep_reduce: atomic_reduce FF (~~ TT).
-
-End ReduceFalse.
-
-Module ReduceTrue.
-
-Inductive atomic_reduce {L: Language} {nL: NormalLanguage L} {pL: PropositionalLanguage L}: expr -> expr -> Prop :=
-| truep_reduce: atomic_reduce TT (FF --> FF).
-
-End ReduceTrue.
-
-Definition MendelsonReduction {L: Language} {nL: NormalLanguage L} {pL: PropositionalLanguage L}: SyntacticReduction L :=
-  Build_SyntacticReduction _
-    (relation_disjunction
-       ImpNegAsPrime.atomic_reduce
-       (relation_disjunction
-         ReduceIff.atomic_reduce
-         ReduceFalse.atomic_reduce)).
-
-Definition IntuitionisticReduction {L: Language} {nL: NormalLanguage L} {pL: PropositionalLanguage L}: SyntacticReduction L :=
-  Build_SyntacticReduction _
-    (relation_disjunction
-       ImpAndOrAsPrime.atomic_reduce
-       (relation_disjunction
-         ReduceIff.atomic_reduce
-         ReduceTrue.atomic_reduce)).
-
 Definition orp_witnessed {L: Language} {nL: NormalLanguage L} {pL: PropositionalLanguage L} {Gamma: ProofTheory L}: context -> Prop :=
   fun Phi => forall x y, Phi (x || y) -> Phi x \/ Phi y.
 
@@ -177,169 +31,19 @@ Inductive expr {Var: Type}: Type :=
   | andp : expr -> expr -> expr
   | orp : expr -> expr -> expr
   | impp : expr -> expr -> expr
-  | iffp : expr -> expr -> expr
-  | negp : expr -> expr
-  | truep : expr
   | falsep : expr
   | varp : Var -> expr.
 
 Implicit Arguments expr.
 
-Inductive single_propagation {Var: Type}: Type :=
-  | and1_propag : expr Var -> single_propagation
-  | and2_propag : expr Var -> single_propagation
-  | or1_propag : expr Var -> single_propagation
-  | or2_propag : expr Var -> single_propagation
-  | imp1_propag : expr Var -> single_propagation
-  | imp2_propag : expr Var -> single_propagation
-  | iff1_propag : expr Var -> single_propagation
-  | iff2_propag : expr Var -> single_propagation
-  | neg_propag : single_propagation
-.
-
-Implicit Arguments single_propagation.
-
-Definition single_propagation_denote {Var: Type} (sp: single_propagation Var) (x: expr Var): expr Var :=
-  match sp with
-  | and1_propag y => andp x y
-  | and2_propag y => andp y x
-  | or1_propag y => orp x y
-  | or2_propag y => orp y x
-  | imp1_propag y => impp x y
-  | imp2_propag y => impp y x
-  | iff1_propag y => iffp x y
-  | iff2_propag y => iffp y x
-  | neg_propag => negp x
-  end.
-
 Instance L (Var: Type): Language :=
-  Build_Language (expr Var) (single_propagation Var) single_propagation_denote.
+  Build_Language (expr Var).
 
 Instance nL (Var: Type): NormalLanguage (L Var) :=
-  Build_NormalLanguage (L Var) falsep impp imp1_propag imp2_propag (fun _ _ => eq_refl) (fun _ _ => eq_refl).
+  Build_NormalLanguage (L Var) falsep impp.
 
 Instance pL (Var: Type): PropositionalLanguage (L Var) :=
-  Build_PropositionalLanguage (L Var) (nL Var) andp orp iffp negp truep
-    and1_propag and2_propag or1_propag or2_propag iff1_propag iff2_propag neg_propag
-    (fun _ _ => eq_refl) (fun _ _ => eq_refl) (fun _ _ => eq_refl) (fun _ _ => eq_refl)
-    (fun _ _ => eq_refl) (fun _ _ => eq_refl) (fun _ => eq_refl).
-
-Definition mendelson_andp {Var: Type} (x y: expr Var): expr Var := negp (impp x (negp y)).
-
-Definition mendelson_orp {Var: Type} (x y: expr Var): expr Var := impp (negp x) y.
-
-Definition mendelson_iffp {Var: Type} (x y: expr Var): expr Var := mendelson_andp (impp x y) (impp y x).
-
-Fixpoint mendelson_reduce {Var: Type} (x: expr Var): expr Var :=
-  match x with
-  | andp y z => mendelson_andp (mendelson_reduce y) (mendelson_reduce z)
-  | orp y z => mendelson_orp (mendelson_reduce y) (mendelson_reduce z)
-  | impp y z => impp (mendelson_reduce y) (mendelson_reduce z)
-  | iffp y z => mendelson_iffp (mendelson_reduce y) (mendelson_reduce z)
-  | negp y => negp (mendelson_reduce y)
-  | truep => truep
-  | falsep => negp truep
-  | varp p => varp p
-  end.
-
-Fixpoint mendelson_normal_form {Var: Type} (x: expr Var): Prop :=
-  match x with
-  | andp y z => False
-  | orp y z => False
-  | impp y z => mendelson_normal_form y /\ mendelson_normal_form z
-  | iffp y z => False
-  | negp y => mendelson_normal_form y
-  | truep => True
-  | falsep => False
-  | varp p => True
-  end.
-
-Definition nMendelsonReduction {Var: Type}: NormalSyntacticReduction (L Var) MendelsonReduction.
-  refine (Build_NormalSyntacticReduction (L Var) _ mendelson_normal_form _).
-  intros; exists (mendelson_reduce x); split.
-  + induction x.
-    - simpl; unfold mendelson_andp.
-      eapply reduce_trans.
-      * apply (@and_reduce (L Var) (nL Var) (pL Var) MendelsonReduction _ _ _ _ IHx1 IHx2).
-      * apply reduce_step.
-        left; apply @ImpNegAsPrime.andp_reduce.
-    - simpl; unfold mendelson_orp.
-      eapply reduce_trans.
-      * apply (@or_reduce (L Var) (nL Var) (pL Var) MendelsonReduction _ _ _ _ IHx1 IHx2).
-      * apply reduce_step.
-        left; apply @ImpNegAsPrime.orp_reduce.
-    - simpl.
-      apply (@imp_reduce (L Var) (nL Var) MendelsonReduction _ _ _ _ IHx1 IHx2).
-    - simpl; unfold mendelson_iffp, mendelson_andp.
-      eapply reduce_trans; [| eapply reduce_trans].
-      * apply (@iff_reduce (L Var) (nL Var) (pL Var) MendelsonReduction _ _ _ _ IHx1 IHx2).
-      * apply reduce_step.
-        right; left; apply @ReduceIff.iff_reduce.
-      * simpl.
-        apply reduce_step.
-        left; apply @ImpNegAsPrime.andp_reduce.
-    - simpl.
-      apply (@neg_reduce (L Var) (nL Var) (pL Var) MendelsonReduction _ _ IHx).
-    - apply reduce_refl.
-    - apply reduce_step.
-      right; right; apply @ReduceFalse.falsep_reduce.
-    - apply reduce_refl.
-  + induction x; simpl; auto.
-Defined.
-
-Definition intuitionistic_iffp {Var: Type} (x y: expr Var): expr Var := andp (impp x y) (impp y x).
-
-Definition intuitionistic_negp {Var: Type} (x: expr Var): expr Var := impp x falsep.
-
-Fixpoint intuitionistic_reduce {Var: Type} (x: expr Var): expr Var :=
-  match x with
-  | andp y z => andp (intuitionistic_reduce y) (intuitionistic_reduce z)
-  | orp y z => orp (intuitionistic_reduce y) (intuitionistic_reduce z)
-  | impp y z => impp (intuitionistic_reduce y) (intuitionistic_reduce z)
-  | iffp y z => intuitionistic_iffp (intuitionistic_reduce y) (intuitionistic_reduce z)
-  | negp y => intuitionistic_negp (intuitionistic_reduce y)
-  | truep => impp falsep falsep
-  | falsep => falsep
-  | varp p => varp p
-  end.
-
-Fixpoint intuitionistic_normal_form {Var: Type} (x: expr Var): Prop :=
-  match x with
-  | andp y z => intuitionistic_normal_form y /\ intuitionistic_normal_form z
-  | orp y z => intuitionistic_normal_form y /\ intuitionistic_normal_form z
-  | impp y z => intuitionistic_normal_form y /\ intuitionistic_normal_form z
-  | iffp y z => False
-  | negp y => False
-  | truep => False
-  | falsep => True
-  | varp p => True
-  end.
-
-Definition nIntuitionisticReduction {Var: Type}: NormalSyntacticReduction (L Var) IntuitionisticReduction.
-  refine (Build_NormalSyntacticReduction (L Var) _ intuitionistic_normal_form _).
-  intros; exists (intuitionistic_reduce x); split.
-  + induction x.
-    - simpl.
-      apply (@and_reduce (L Var) (nL Var) (pL Var) IntuitionisticReduction _ _ _ _ IHx1 IHx2).
-    - apply (@or_reduce (L Var) (nL Var) (pL Var) IntuitionisticReduction _ _ _ _ IHx1 IHx2).
-    - simpl.
-      apply (@imp_reduce (L Var) (nL Var) IntuitionisticReduction _ _ _ _ IHx1 IHx2).
-    - simpl; unfold intuitionistic_iffp.
-      eapply reduce_trans.
-      * apply (@iff_reduce (L Var) (nL Var) (pL Var) IntuitionisticReduction _ _ _ _ IHx1 IHx2).
-      * apply reduce_step.
-        right. left. apply @ReduceIff.iff_reduce.
-    - simpl; unfold intuitionistic_negp.
-      eapply reduce_trans.
-      * apply (@neg_reduce (L Var) (nL Var) (pL Var) IntuitionisticReduction _ _ IHx).
-      * apply reduce_step.
-        left. apply @ImpAndOrAsPrime.negp_reduce.
-    - apply reduce_step.
-      right. right. apply @ReduceTrue.truep_reduce.
-    - apply reduce_refl.
-    - apply reduce_refl.
-  + induction x; simpl; auto.
-Defined.
+  Build_PropositionalLanguage (L Var) (nL Var) andp orp.
 
 Definition rank {Var: Type}: expr Var -> nat :=
   fix rank (x: expr Var): nat :=
@@ -347,9 +51,6 @@ Definition rank {Var: Type}: expr Var -> nat :=
     | andp y z => 1 + rank y + rank z
     | orp y z => 1 + rank y + rank z
     | impp y z => 1 + rank y + rank z
-    | iffp y z => 1 + rank y + rank z
-    | negp y => 1 + rank y
-    | truep => 0
     | falsep => 0
     | varp p => 0
     end.
@@ -358,89 +59,63 @@ Definition formula_countable: forall Var, Countable Var -> Countable (expr Var).
   intros.
   assert (forall n, Countable (sig (fun x: expr Var => rank x <= n))).
   + induction n.
-    - apply (@bijection_Countable _ (Var + unit + unit)%type); [| solve_Countable].
+    - apply (@bijection_Countable _ (Var + unit)%type); [| solve_Countable].
       apply bijection_sym.
       apply (FBuild_bijection _ _ (fun x =>
                match x with
-               | inl (inl p) => exist (fun x: expr Var => rank x <= 0) (varp p) (le_n 0)
-               | inl (inr _) => exist (fun x: expr Var => rank x <= 0) truep (le_n 0)
+               | inl p => exist (fun x: expr Var => rank x <= 0) (varp p) (le_n 0)
                | inr _ => exist (fun x: expr Var => rank x <= 0) falsep (le_n 0)
                end)).
       * hnf; intros.
-        destruct a1 as [[? | []] | []], a2 as [[? | []] | []]; inversion H; auto.
+        destruct a1 as [? | []], a2 as [? | []]; inversion H; auto.
       * hnf; intros.
         destruct b as [[] HH]; try solve [inversion HH].
-        1: exists (inl (inr tt)); eauto; f_equal; apply proof_irrelevance.
         1: exists (inr tt); eauto; f_equal; apply proof_irrelevance.
-        1: exists (inl (inl v)); eauto; f_equal; apply proof_irrelevance.
+        1: exists (inl v); eauto; f_equal; apply proof_irrelevance.
     - set (s := sig (fun x: expr Var => rank x <= n)).
-      apply (@injection_Countable _ (s * s + s * s + s * s + s * s + s + unit + unit + Var)%type); [| solve_Countable].
+      apply (@injection_Countable _ (s * s + s * s + s * s + unit + Var)%type); [| solve_Countable].
       apply (Build_injection _ _ (fun x y =>
         match y with
-        | inl (inl (inl (inl (inl (inl (inl (exist y _, exist z _))))))) => proj1_sig x = andp y z
-        | inl (inl (inl (inl (inl (inl (inr (exist y _, exist z _))))))) => proj1_sig x = orp y z
-        | inl (inl (inl (inl (inl (inr (exist y _, exist z _)))))) => proj1_sig x = impp y z
-        | inl (inl (inl (inl (inr (exist y _, exist z _))))) => proj1_sig x = iffp y z
-        | inl (inl (inl (inr (exist y _)))) => proj1_sig x = negp y
-        | inl (inl (inr _)) => proj1_sig x = truep
+        | inl (inl (inl (inl (exist y _, exist z _)))) => proj1_sig x = andp y z
+        | inl (inl (inl (inr (exist y _, exist z _)))) => proj1_sig x = orp y z
+        | inl (inl (inr (exist y _, exist z _))) => proj1_sig x = impp y z
         | inl (inr _) => proj1_sig x = falsep
         | inr p => proj1_sig x = varp p
         end)).
       * hnf; intros.
-        destruct a as [[y z | y z | y z | y z | y | | | p] ?H].
+        destruct a as [[y z | y z | y z | | p] ?H].
         (* 1 *) simpl in H. assert (rank y <= n) by omega. assert (rank z <= n) by omega.
-                exists (inl (inl (inl (inl (inl (inl (inl (exist _ y H0, exist _ z H1)))))))); auto.
+                exists (inl (inl (inl (inl (exist _ y H0, exist _ z H1))))); auto.
         (* 2 *) simpl in H. assert (rank y <= n) by omega. assert (rank z <= n) by omega.
-                exists (inl (inl (inl (inl (inl (inl (inr (exist _ y H0, exist _ z H1)))))))); auto.
+                exists (inl (inl (inl (inr (exist _ y H0, exist _ z H1))))); auto.
         (* 3 *) simpl in H. assert (rank y <= n) by omega. assert (rank z <= n) by omega.
-                exists (inl (inl (inl (inl (inl (inr (exist _ y H0, exist _ z H1))))))); auto.
-        (* 4 *) simpl in H. assert (rank y <= n) by omega. assert (rank z <= n) by omega.
-                exists (inl (inl (inl (inl (inr (exist _ y H0, exist _ z H1)))))); auto.
-        (* 5 *) simpl in H. assert (rank y <= n) by omega.
-                exists (inl (inl (inl (inr (exist _ y H0))))); auto.
-        (* 6 *) exists (inl (inl (inr tt))); auto.
-        (* 7 *) exists (inl (inr tt)); auto.
-        (* 8 *) exists (inr p); auto.
+                exists (inl (inl (inr (exist _ y H0, exist _ z H1)))); auto.
+        (* 4 *) exists (inl (inr tt)); auto.
+        (* 5 *) exists (inr p); auto.
       * hnf; intros.
-        destruct a as [[y z | y z | y z | y z | y | | | p] ?H];
-        destruct b1 as [[[[[[[[[y1 ?H] [z1 ?H]] | [[y1 ?H] [z1 ?H]]] | [[y1 ?H] [z1 ?H]]] | [[y1 ?H] [z1 ?H]]]| [y1 ?]]| ] |] | p1]; try solve [inversion H];
-        destruct b2 as [[[[[[[[[y2 ?H] [z2 ?H]] | [[y2 ?H] [z2 ?H]]] | [[y2 ?H] [z2 ?H]]] | [[y2 ?H] [z2 ?H]]]| [y2 ?]]| ] |] | p2]; try solve [inversion H0].
+        destruct a as [[y z | y z | y z | | p] ?H];
+        destruct b1 as [[[[[[y1 ?H] [z1 ?H]] | [[y1 ?H] [z1 ?H]]] | [[y1 ?H] [z1 ?H]]] |] | p1]; try solve [inversion H];
+        destruct b2 as [[[[[[y2 ?H] [z2 ?H]] | [[y2 ?H] [z2 ?H]]] | [[y2 ?H] [z2 ?H]]] |] | p2]; try solve [inversion H0].
         (* 1 *) inversion H; inversion H0; subst; subst; repeat f_equal; apply proof_irrelevance.
         (* 2 *) inversion H; inversion H0; subst; subst; repeat f_equal; apply proof_irrelevance.
         (* 3 *) inversion H; inversion H0; subst; subst; repeat f_equal; apply proof_irrelevance.
-        (* 4 *) inversion H; inversion H0; subst; subst; repeat f_equal; apply proof_irrelevance.
+        (* 4 *) destruct u, u0; auto.
         (* 5 *) inversion H; inversion H0; subst; subst; repeat f_equal; apply proof_irrelevance.
-        (* 6 *) destruct u, u0; auto.
-        (* 7 *) destruct u, u0; auto.
-        (* 8 *) inversion H; inversion H0; subst; subst; repeat f_equal; apply proof_irrelevance.
       * hnf; intros.
-        destruct b as [[[[[[[[[y ?H] [z ?H]] | [[y ?H] [z ?H]]] | [[y ?H] [z ?H]]] | [[y ?H] [z ?H]]]| [y ?]]| ] |] | p];
-        destruct a1 as [[y1 z1 | y1 z1 | y1 z1 | y1 z1 | y1 | | | p1] ?H]; try solve [inversion H];
-        destruct a2 as [[y2 z2 | y2 z2 | y2 z2 | y2 z2 | y2 | | | p2] ?H]; try solve [inversion H0].
+        destruct b as [[[[[[y ?H] [z ?H]] | [[y ?H] [z ?H]]] | [[y ?H] [z ?H]]] |] | p];
+        destruct a1 as [[y1 z1 | y1 z1 | y1 z1 | | p1] ?H]; try solve [inversion H];
+        destruct a2 as [[y2 z2 | y2 z2 | y2 z2 | | p2] ?H]; try solve [inversion H0].
         (* 1 *) inversion H; inversion H0; subst; subst; repeat f_equal; apply proof_irrelevance.
         (* 2 *) inversion H; inversion H0; subst; subst; repeat f_equal; apply proof_irrelevance.
         (* 3 *) inversion H; inversion H0; subst; subst; repeat f_equal; apply proof_irrelevance.
-        (* 4 *) inversion H; inversion H0; subst; subst; repeat f_equal; apply proof_irrelevance.
+        (* 4 *) f_equal; apply proof_irrelevance.
         (* 5 *) inversion H; inversion H0; subst; subst; repeat f_equal; apply proof_irrelevance.
-        (* 6 *) f_equal; apply proof_irrelevance.
-        (* 7 *) f_equal; apply proof_irrelevance.
-        (* 8 *) inversion H; inversion H0; subst; subst; repeat f_equal; apply proof_irrelevance.
   + apply (@injection_Countable _ (sigT (fun n => sig (fun x: expr Var => rank x <= n)))); [| solve_Countable; auto].
     apply (FBuild_injection _ _ (fun x => existT _ (rank x) (exist _ x (le_n _)))).
     hnf; intros.
     simpl in H.
     inversion H; auto.
 Qed. (* 20 seconds *)
-
-Lemma RPPC_RPC {Var} {Gamma: ProofTheory (L Var)}:
-  PropositonalPropagationConsistentProvable Gamma ->
-  ReductionPropagationConsistentProvable Gamma.
-Proof.
-  intros.
-  hnf; intros.
-  apply (H x y sp); auto.
-  destruct sp; constructor.
-Qed.
 
 End PropositionalLanguage.
 
