PropositionalLogic/TrivialSemantics.v
@@ -1,24 +1,17 @@
 Require Import Coq.Logic.Classical_Prop.
 Require Import Logic.LogicBase.
 Require Import Logic.MinimunLogic.MinimunLogic.
-Require Import Logic.MinimunLogic.SyntacticReduction.
 Require Import Logic.PropositionalLogic.Syntax.
 
 Local Open Scope logic_base.
 Local Open Scope PropositionalLogic.
 
-Class TrivialPropositionalSemantics (L: Language) {nL: NormalLanguage L} {pL: PropositionalLanguage L} (SM: Semantics L) {mcSM: ReductionConsistentSemantics MendelsonReduction SM}: Type := {
+Class TrivialPropositionalSemantics (L: Language) {nL: NormalLanguage L} {pL: PropositionalLanguage L} (SM: Semantics L): Type := {
+  sat_andp: forall m x y, m |= x && y <-> (m |= x /\ m |= y);
+  sat_orp: forall m x y, m |= x || y <-> (m |= x \/ m |= y);
   sat_impp: forall m x y, m |= x --> y <-> (m |= x -> m |= y);
-  sat_negp: forall m x, m |= ~~ x <-> ~ m |= x;
-  sat_truep: forall m, m |= TT
+  sat_falsep: forall m, ~ m |= FF
 }.
-
-(*
-  sem_falsep: forall m, ~ m |= FF;
-  sem_andp: forall m x y, m |= x && y <-> m |= ~~ (x --> ~~ y);
-  sem_orp: forall m x y, m |= x || y <-> m |= ~~ x --> y;
-  sem_iffp: forall m x y, m |= (x <--> y) <-> m |= (x --> y) && (y --> x)
-*)
 
 Module TrivialSemantics.
 
@@ -29,26 +22,17 @@ Definition model (Var: Type): Type := Var -> Prop.
 Definition sem_imp {model: Type} (X: Ensemble model) (Y: Ensemble model): Ensemble model :=
   fun m => X m -> Y m.
 
-Definition sem_neg {model: Type} (X: Ensemble model): Ensemble model :=
-  fun m => ~ X m.
-
 Definition sem_and {model: Type} (X: Ensemble model) (Y: Ensemble model): Ensemble model :=
-  sem_neg (sem_imp X (sem_neg Y)).
+  fun m => X m /\ Y m.
 
 Definition sem_or {model: Type} (X: Ensemble model) (Y: Ensemble model): Ensemble model :=
-  sem_imp (sem_neg X) Y.
-
-Definition sem_iff {model: Type} (X: Ensemble model) (Y: Ensemble model): Ensemble model :=
-  sem_and (sem_imp X Y) (sem_imp Y X).
+  fun m => X m \/ Y m.
 
 Fixpoint denotation {Var: Type} (x: expr Var): Ensemble (model Var) :=
   match x with
   | andp y z => sem_and (denotation y) (denotation z)
   | orp y z => sem_or (denotation y) (denotation z)
   | impp y z => sem_imp (denotation y) (denotation z)
-  | iffp y z => sem_iff (denotation y) (denotation z)
-  | negp y => sem_neg (denotation y)
-  | truep => fun _ => True
   | falsep => fun _ => False
   | varp p => fun m => m p
   end.
@@ -56,87 +40,15 @@ Fixpoint denotation {Var: Type} (x: expr Var): Ensemble (model Var) :=
 Instance SM (Var: Type): Semantics (PropositionalLanguage.L Var) :=
   Build_Semantics (PropositionalLanguage.L Var) (model Var) (fun m x => denotation x m).
 
-Lemma ImpNegAsPrime_consistent {Var: Type}:
-  forall x y: expr Var,
-    @ImpNegAsPrime.atomic_reduce (L Var) (nL Var) (pL Var) x y ->
-    forall m: model Var, denotation x m <-> denotation y m.
-Proof.
-  intros; split; intros; destruct H; auto.
-Qed.
-
-Lemma ReduceIff_consistent {Var: Type}:
-  forall x y: expr Var,
-    @ReduceIff.atomic_reduce (L Var) (nL Var) (pL Var) x y ->
-    forall m: model Var, denotation x m <-> denotation y m.
-Proof.
-  intros; split; intros; destruct H; auto.
-Qed.
-
-Lemma ReduceFalse_consistent {Var: Type}:
-  forall x y: expr Var,
-    @ReduceFalse.atomic_reduce (L Var) (nL Var) (pL Var) x y ->
-    forall m: model Var, denotation x m <-> denotation y m.
-Proof.
-  intros; split; intros; destruct H.
-  + simpl in H0.
-    inversion H0.
-  + specialize (H0 I).
-    inversion H0.
-Qed.
-
-Lemma RPC {Var: Type}: ReductionPropagationConsistentSemantics (SM Var).
-Proof.
-  hnf; intros; simpl in *.
-  specialize (H m).
-  destruct sp.
-  + simpl in *.
-    unfold TrivialSemantics.sem_and, TrivialSemantics.sem_neg, TrivialSemantics.sem_imp; simpl.
-    tauto.
-  + simpl in *.
-    unfold TrivialSemantics.sem_and, TrivialSemantics.sem_neg, TrivialSemantics.sem_imp; simpl.
-    tauto.
-  + simpl in *.
-    unfold TrivialSemantics.sem_or, TrivialSemantics.sem_neg, TrivialSemantics.sem_imp; simpl.
-    tauto.
-  + simpl in *.
-    unfold TrivialSemantics.sem_or, TrivialSemantics.sem_neg, TrivialSemantics.sem_imp; simpl.
-    tauto.
-  + simpl in *.
-    unfold TrivialSemantics.sem_imp; simpl.
-    tauto.
-  + simpl in *.
-    unfold TrivialSemantics.sem_imp; simpl.
-    tauto.
-  + simpl in *.
-    unfold TrivialSemantics.sem_iff, TrivialSemantics.sem_and, TrivialSemantics.sem_neg, TrivialSemantics.sem_imp; simpl.
-    tauto.
-  + simpl in *.
-    unfold TrivialSemantics.sem_iff, TrivialSemantics.sem_and, TrivialSemantics.sem_neg, TrivialSemantics.sem_imp; simpl.
-    tauto.
-  + simpl in *.
-    unfold TrivialSemantics.sem_neg; simpl.
-    tauto.
-Qed.
-
-Instance mcSM (Var: Type): ReductionConsistentSemantics MendelsonReduction (SM Var).
-Proof.
-  apply Build_ReductionConsistentSemantics.
-  + hnf; intros.
-    revert x y H m.
-    repeat apply disjunction_reduce_consistent_semantics.
-    - apply ImpNegAsPrime_consistent.
-    - apply ReduceIff_consistent.
-    - apply ReduceFalse_consistent.
-  + apply RPC.
-Qed.
-
 Instance tpSM (Var: Type): TrivialPropositionalSemantics (L Var) (SM Var).
 Proof.
   constructor.
   + simpl; intros.
-    unfold sem_imp; tauto.
+    unfold sem_and; tauto.
   + simpl; intros.
-    unfold sem_neg; tauto.
+    unfold sem_or; tauto.
+  + simpl; intros.
+    unfold sem_imp; tauto.
   + simpl; intros; auto.
 Qed.
 
