Makefile
@@ -4,11 +4,12 @@ COQC = coqc
 	@echo COQC $*.v
 	@$(COQC) -q -R "." -as Logic $*.v
 
-all: Wf.vo base.vo IPC.vo trivial.vo Kripke.vo enumerate.vo LogicBase.vo MinimunLogic/SyntacticReduction.v \
+all: Wf.vo base.vo IPC.vo trivial.vo Kripke.vo enumerate.vo LogicBase.vo \
      MinimunLogic/HenkinCompleteness.v MinimunLogic/MinimunLogic.vo MinimunLogic/ContextProperty.vo \
      PropositionalLogic/IntuitionisticPropositionalLogic.vo \
      PropositionalLogic/KripkeSemantics.vo \
      PropositionalLogic/Syntax.vo PropositionalLogic/ClassicalPropositionalLogic.vo \
      PropositionalLogic/TrivialSemantics.vo PropositionalLogic/Sound_Classical_Trivial.vo \
      PropositionalLogic/Complete_Classical_Trivial.vo lib/Coqlib.vo \
-     lib/Bijection.vo lib/Countable.vo PropositionalLogic/Complete_Intuitionistic_Kripke.vo 
+     lib/Bijection.vo lib/Countable.vo PropositionalLogic/Complete_Intuitionistic_Kripke.vo \
+     PropositionalLogic/CanonicalKripke.vo 
